Added BinaryTree and List data types

src/data-types/list/List.dfy
@@ -1,17 +1,18 @@
 type T = int
 
-datatype List<T> = Nil | Cons(head:T, tail:List<T>)
+datatype List_Empty = Nil
+datatype List<T> = List_Empty | Cons(head:T, tail:List<T>)
 
 function create(): List<T>
 {
-  Nil
+  List_Empty
 }
 
 function method List_Insert(a:List<T>, x:T) : List<T>
   decreases a
 {
   match a {
-    case Nil => Cons(x, Nil)
+    case List_Empty => Cons(x, List_Empty)
     case Cons(h, t) => Cons(h, List_Insert(t, x))
   }
 }
@@ -20,17 +21,33 @@ function method List_Concat(a:List<T>, b:List<T>) : List<T>
   decreases a
 {
   match a {
-    case Nil => b
+    case List_Empty => b
     case Cons(h, t) => Cons(h, List_Concat(t, b))
   }
 }
 
-method List_Print(a:List<T>) {
+function List_Head(xs:List<T>): T
+  requires xs != List_Empty
+{
+  match xs
+    case Cons(y, ys) => y
+}
+
+function List_Tail(xs:List<T>): List<T>
+{
+  match xs
+    case List_Empty => List_Empty
+    case Cons(y, ys) => ys
+}
+
+method List_Print(a:List<T>) 
+  decreases a
+{
   match a {
-    case Nil => {
+    case List_Empty => {
       return;
     }
-    case Cons(h, Nil) => {
+    case Cons(h, List_Empty) => {
       print h, "\n";
       return;
     }
