src/data-types/binary-tree/BinaryTree.dfy
@@ -1,20 +1,25 @@
-type T = int
+include "../list/List.dfy"
 
-datatype BinaryTree<T> = Leaf(data:T) | Node(left:BinaryTree<T>, data:T, right:BinaryTree<T>)
+datatype Leaf = Nil
+datatype BinaryTree<T> = Leaf | Node(left:BinaryTree<T>, data:T, right:BinaryTree<T>)
 
-function elems(tree: BinaryTree<T>): set<T>
-    decreases tree
+function method BinaryTree_InOrderElems(tree:BinaryTree<T>) : List<T>
+  decreases tree
 {
-    match tree
-        case Leaf => {}
-        case Node(left, data, right) => elems(left) + {data} + elems(right)
+  match tree {
+    case Leaf => List_Empty
+    case Node(l, d, r) => List_Concat(BinaryTree_InOrderElems(l), List_Concat(Cons(d, List_Empty), BinaryTree_InOrderElems(r)))
+  }
 }
 
-function descendants(tree: BinaryTree<T>) : set<BinaryTree<T>>
-    decreases tree
+function method BinaryTree_Insert(tree:BinaryTree<T>, x:int): BinaryTree<T>
+  decreases tree
 {
-    match tree {
-        case Leaf => {}
-        case Node(left, _, right) => descendants(left) + descendants(right)
-    }
+  match tree {
+    case Leaf => Node(Leaf, x, Leaf)
+    case Node(l, d, r) => 
+      if (x < d) then Node(BinaryTree_Insert(l, x), d, r)
+      else if (x > d) then Node(l, d, BinaryTree_Insert(r, x))
+      else tree
+  }
 }
