test/data-types/binary-tree/BinaryTreeTest.dfy
@@ -1,0 +1,36 @@
+include "../../../src/data-types/binary-tree/BinaryTree.dfy"
+
+method Main() {
+  InOrderElemsTest();
+  InsertTest();
+  InsertWorstCaseTest();
+}
+
+method InOrderElemsTest() {
+  var tree: BinaryTree<int> := Node(Node(Node(Leaf,1,Leaf),3,Leaf),4,Node(Node(Leaf, 5, Leaf),7,Leaf));
+  var list := BinaryTree_InOrderElems(tree);
+  var expected := Cons(1, Cons(3, Cons(4, Cons(5, Cons(7, List_Empty)))));
+  assert(list == expected);
+}
+
+method InsertTest() {
+  var tree: BinaryTree<int> := Leaf;
+  tree := BinaryTree_Insert(tree, 4);
+  tree := BinaryTree_Insert(tree, 3);
+  tree := BinaryTree_Insert(tree, 1);
+  tree := BinaryTree_Insert(tree, 7);
+  tree := BinaryTree_Insert(tree, 5);
+  var expected := Node(Node(Node(Leaf,1,Leaf),3,Leaf),4,Node(Node(Leaf, 5, Leaf),7,Leaf));
+  assert(tree == expected);
+}
+
+method InsertWorstCaseTest() {
+  var tree: BinaryTree<int> := Leaf;
+  tree := BinaryTree_Insert(tree, 1);
+  tree := BinaryTree_Insert(tree, 3);
+  tree := BinaryTree_Insert(tree, 4);
+  tree := BinaryTree_Insert(tree, 5);
+  tree := BinaryTree_Insert(tree, 7);
+  var expected := Node(Leaf, 1, Node(Leaf, 3, Node(Leaf, 4, Node(Leaf, 5, Node(Leaf, 7, Leaf)))));
+  assert(tree == expected);
+}
