test/data-types/list/ListTest.dfy
@@ -6,26 +6,26 @@ method Main() {
 }
 
 method InsertIntoListTest() {
-  var list: List<int> := Nil;
+  var list: List<int> := List_Empty;
   list := List_Insert(list, 2);
   list := List_Insert(list, 10);
   list := List_Insert(list, 4);
   list := List_Insert(list, 12);
   list := List_Insert(list, 7);
 
-  assert(list == Cons(2, Cons(10, Cons(4, Cons(12, Cons(7, Nil))))));
+  assert(list == Cons(2, Cons(10, Cons(4, Cons(12, Cons(7, List_Empty))))));
 }
 
 method ConcatTwoListsTest() {
-  var a: List<int> := Nil;
+  var a: List<int> := List_Empty;
   a := List_Insert(a, 2);
   a := List_Insert(a, 10);
 
-  var b: List<int> := Nil;
+  var b: List<int> := List_Empty;
   b := List_Insert(b, 4);
   b := List_Insert(b, 12);
   b := List_Insert(b, 7);
 
   var c := List_Concat(a, b);
-  assert(c == Cons(2, Cons(10, Cons(4, Cons(12, Cons(7, Nil))))));
+  assert(c == Cons(2, Cons(10, Cons(4, Cons(12, Cons(7, List_Empty))))));
 }
